Add double tree rotations

examples/steel/Selectors.Tree.fst
@@ -136,4 +136,130 @@ let rotate_right #a ptr =
       (get_left x_node)
     )
   )
+
+let rotate_right_left #a ptr =
+  let h = get #(linked_tree ptr) () in
+
+  // if top pointer is null
+  if is_null_t ptr then (
+    elim_linked_tree_leaf ptr;
+    assert(Spec.rotate_right_left (v_linked_tree ptr h) == None);
+    assert(False);
+    noop ();
+    ptr
+  ) else (
+
+    // original root node
+    let x_node = unpack_tree ptr in
+    let x = get_data x_node in
+
+    // if z is null
+    if is_null_t (get_right x_node) then (
+      elim_linked_tree_leaf (get_right x_node);
+      assert(Spec.rotate_right_left (v_linked_tree ptr h) == None);
+      assert(False);
+      pack_tree ptr (get_left x_node) (get_right x_node);
+      ptr
+    ) else (
+    
+      // original right node
+      // z = get_right x_node
+      let z_node = unpack_tree (get_right x_node) in
+      let z = get_data z_node in
+
+      // if y is null
+      if is_null_t (get_left z_node) then (
+        elim_linked_tree_leaf (get_left z_node);
+        assert(Spec.rotate_right_left (v_linked_tree ptr h) == None);
+        assert(False);
+        pack_tree (get_right x_node) (get_left z_node) (get_right z_node);
+        pack_tree ptr (get_left x_node) (get_right x_node);
+        ptr
+      ) else (
+
+        // original left (right node)
+        // y = get_left (z_node)
+        let y_node = unpack_tree (get_left z_node) in
+        let y = get_data y_node in
+
+        let new_x = mk_node x (get_left x_node) (get_left y_node) in
+        let new_z = mk_node z (get_right y_node) (get_right z_node) in
+        let new_y = mk_node y ptr (get_right x_node) in
+
+        write ptr new_x;
+        write (get_right x_node) new_z;
+        write (get_left z_node) new_y;
+
+        pack_tree ptr (get_left x_node) (get_left y_node);
+        pack_tree (get_right x_node) (get_right y_node) (get_right z_node);
+        pack_tree (get_left z_node) ptr (get_right x_node);
+
+        (get_left z_node)
+
+      )
+    )
+  )
+
+let rotate_left_right #a ptr =
+  let h = get #(linked_tree ptr) () in
+
+  // if top pointer is null
+  if is_null_t ptr then (
+    elim_linked_tree_leaf ptr;
+    assert(Spec.rotate_right_left (v_linked_tree ptr h) == None);
+    assert(False);
+    noop ();
+    ptr
+  ) else (
+
+    // original root node
+    let x_node = unpack_tree ptr in
+    let x = get_data x_node in
+
+    // if z is null
+    if is_null_t (get_left x_node) then (
+      elim_linked_tree_leaf (get_left x_node);
+      assert(Spec.rotate_left_right (v_linked_tree ptr h) == None);
+      assert(False);
+      pack_tree ptr (get_left x_node) (get_right x_node);
+      ptr
+    ) else (
+    
+      // original left node
+      // z = get_left x_node
+      let z_node = unpack_tree (get_left x_node) in
+      let z = get_data z_node in
+
+      // if y is null
+      if is_null_t (get_right z_node) then (
+        elim_linked_tree_leaf (get_right z_node);
+        assert(Spec.rotate_left_right (v_linked_tree ptr h) == None);
+        assert(False);
+        pack_tree (get_left x_node) (get_left z_node) (get_right z_node);
+        pack_tree ptr (get_left x_node) (get_right x_node);
+        ptr
+      ) else (
+
+        // original right (left node)
+        // y = get_right (z_node)
+        let y_node = unpack_tree (get_right z_node) in
+        let y = get_data y_node in
+
+        let new_z = mk_node z (get_left z_node) (get_left y_node) in
+        let new_x = mk_node x (get_right y_node) (get_right x_node) in
+        let new_y = mk_node y (get_left x_node) ptr in
+
+        write (get_left x_node) new_z;
+        write ptr new_x;
+        write (get_right z_node) new_y;
+
+        pack_tree (get_left x_node) (get_left z_node) (get_left y_node);
+        pack_tree ptr (get_right y_node) (get_right x_node);
+        pack_tree (get_right z_node) (get_left x_node) ptr;
+
+        (get_right z_node)
+
+      )
+    )
+  )
 #pop-options
